examples/ProcDecSCN.v
@@ -11,23 +11,23 @@ Require Import Ex.ProcDec Ex.ProcDecInl Ex.ProcDecInv Ex.ProcDecSC.
 Set Implicit Arguments.
 
 Section ProcDecSCN.
-  Variables addrSize iaddrSize fifoSize lgDataBytes rfIdx: nat.
+  Variables addrSize iaddrSize fifoSize dataBytes rfIdx: nat.
 
   (* External abstract ISA: decoding and execution *)
-  Variables (getOptype: OptypeT lgDataBytes)
-            (getLdDst: LdDstT lgDataBytes rfIdx)
-            (getLdAddr: LdAddrT addrSize lgDataBytes)
-            (getLdSrc: LdSrcT lgDataBytes rfIdx)
-            (calcLdAddr: LdAddrCalcT addrSize lgDataBytes)
-            (getStAddr: StAddrT addrSize lgDataBytes)
-            (getStSrc: StSrcT lgDataBytes rfIdx)
-            (calcStAddr: StAddrCalcT addrSize lgDataBytes)
-            (getStVSrc: StVSrcT lgDataBytes rfIdx)
-            (getSrc1: Src1T lgDataBytes rfIdx)
-            (getSrc2: Src2T lgDataBytes rfIdx)
-            (getDst: DstT lgDataBytes rfIdx)
-            (exec: ExecT addrSize lgDataBytes)
-            (getNextPc: NextPcT addrSize lgDataBytes rfIdx)
+  Variables (getOptype: OptypeT dataBytes)
+            (getLdDst: LdDstT dataBytes rfIdx)
+            (getLdAddr: LdAddrT addrSize dataBytes)
+            (getLdSrc: LdSrcT dataBytes rfIdx)
+            (calcLdAddr: LdAddrCalcT addrSize dataBytes)
+            (getStAddr: StAddrT addrSize dataBytes)
+            (getStSrc: StSrcT dataBytes rfIdx)
+            (calcStAddr: StAddrCalcT addrSize dataBytes)
+            (getStVSrc: StVSrcT dataBytes rfIdx)
+            (getSrc1: Src1T dataBytes rfIdx)
+            (getSrc2: Src2T dataBytes rfIdx)
+            (getDst: DstT dataBytes rfIdx)
+            (exec: ExecT addrSize dataBytes)
+            (getNextPc: NextPcT addrSize dataBytes rfIdx)
             (alignPc: AlignPcT addrSize iaddrSize).
 
   Variable n: nat.
@@ -53,7 +53,7 @@ Section ProcDecSCN.
   Definition procDecN := pdecs getOptype getLdDst getLdAddr getLdSrc calcLdAddr
                                getStAddr getStSrc calcStAddr getStVSrc
                                getSrc1 getSrc2 getDst exec getNextPc alignPc n.
-  Definition memAtomic := memAtomic addrSize fifoSize lgDataBytes n.
+  Definition memAtomic := memAtomic addrSize fifoSize dataBytes n.
   Definition pdecAN := (procDecN ++ memAtomic)%kami.
 
   Lemma pdecN_memAtomic_refines_scN: pdecAN <<== scN.
