examples/ProcFDCorrect.v
@@ -11,23 +11,23 @@ Require Import Eqdep.
 Set Implicit Arguments.
 
 Section FetchDecode.
-  Variables addrSize iaddrSize lgDataBytes rfIdx: nat.
+  Variables addrSize iaddrSize dataBytes rfIdx: nat.
 
   (* External abstract ISA: decoding and execution *)
-  Variables (getOptype: OptypeT lgDataBytes)
-            (getLdDst: LdDstT lgDataBytes rfIdx)
-            (getLdAddr: LdAddrT addrSize lgDataBytes)
-            (getLdSrc: LdSrcT lgDataBytes rfIdx)
-            (calcLdAddr: LdAddrCalcT addrSize lgDataBytes)
-            (getStAddr: StAddrT addrSize lgDataBytes)
-            (getStSrc: StSrcT lgDataBytes rfIdx)
-            (calcStAddr: StAddrCalcT addrSize lgDataBytes)
-            (getStVSrc: StVSrcT lgDataBytes rfIdx)
-            (getSrc1: Src1T lgDataBytes rfIdx)
-            (getSrc2: Src2T lgDataBytes rfIdx)
-            (getDst: DstT lgDataBytes rfIdx)
-            (exec: ExecT addrSize lgDataBytes)
-            (getNextPc: NextPcT addrSize lgDataBytes rfIdx)
+  Variables (getOptype: OptypeT dataBytes)
+            (getLdDst: LdDstT dataBytes rfIdx)
+            (getLdAddr: LdAddrT addrSize dataBytes)
+            (getLdSrc: LdSrcT dataBytes rfIdx)
+            (calcLdAddr: LdAddrCalcT addrSize dataBytes)
+            (getStAddr: StAddrT addrSize dataBytes)
+            (getStSrc: StSrcT dataBytes rfIdx)
+            (calcStAddr: StAddrCalcT addrSize dataBytes)
+            (getStVSrc: StVSrcT dataBytes rfIdx)
+            (getSrc1: Src1T dataBytes rfIdx)
+            (getSrc2: Src2T dataBytes rfIdx)
+            (getDst: DstT dataBytes rfIdx)
+            (exec: ExecT addrSize dataBytes)
+            (getNextPc: NextPcT addrSize dataBytes rfIdx)
             (alignPc: AlignPcT addrSize iaddrSize)
             (predictNextPc: forall ty, fullType ty (SyntaxKind (Bit addrSize)) -> (* pc *)
                                        Expr ty (SyntaxKind (Bit addrSize))).
@@ -38,9 +38,9 @@ Section FetchDecode.
                 Expr ty (SyntaxKind (Bit 2)) -> (* opTy *)
                 Expr ty (SyntaxKind (Bit rfIdx)) -> (* dst *)
                 Expr ty (SyntaxKind (Bit addrSize)) -> (* addr *)
-                Expr ty (SyntaxKind (Data lgDataBytes)) -> (* val1 *)
-                Expr ty (SyntaxKind (Data lgDataBytes)) -> (* val2 *)
-                Expr ty (SyntaxKind (Data lgDataBytes)) -> (* rawInst *)
+                Expr ty (SyntaxKind (Data dataBytes)) -> (* val1 *)
+                Expr ty (SyntaxKind (Data dataBytes)) -> (* val2 *)
+                Expr ty (SyntaxKind (Data dataBytes)) -> (* rawInst *)
                 Expr ty (SyntaxKind (Bit addrSize)) -> (* curPc *)
                 Expr ty (SyntaxKind (Bit addrSize)) -> (* nextPc *)
                 Expr ty (SyntaxKind Bool) -> (* epoch *)
@@ -49,14 +49,14 @@ Section FetchDecode.
   Variable (f2dElt: Kind).
   Variable (f2dPack:
               forall ty,
-                Expr ty (SyntaxKind (Data lgDataBytes)) -> (* rawInst *)
+                Expr ty (SyntaxKind (Data dataBytes)) -> (* rawInst *)
                 Expr ty (SyntaxKind (Bit addrSize)) -> (* curPc *)
                 Expr ty (SyntaxKind (Bit addrSize)) -> (* nextPc *)
                 Expr ty (SyntaxKind Bool) -> (* epoch *)
                 Expr ty (SyntaxKind f2dElt)).
   Variables
     (f2dRawInst: forall ty, fullType ty (SyntaxKind f2dElt) ->
-                            Expr ty (SyntaxKind (Data lgDataBytes)))
+                            Expr ty (SyntaxKind (Data dataBytes)))
     (f2dCurPc: forall ty, fullType ty (SyntaxKind f2dElt) ->
                           Expr ty (SyntaxKind (Bit addrSize)))
     (f2dNextPc: forall ty, fullType ty (SyntaxKind f2dElt) ->
@@ -101,7 +101,7 @@ Section FetchDecode.
 
   Definition fetchDecode_regMap (r: RegsT): RegsT :=
     (mlet pcv : (Bit addrSize) <- r |> "pc";
-       mlet pgmv : (Vector (Data lgDataBytes) iaddrSize) <- r |> "pgm";
+       mlet pgmv : (Vector (Data dataBytes) iaddrSize) <- r |> "pgm";
        mlet fev : Bool <- r |> "fEpoch";
        mlet f2dfullv : Bool <- r |> "f2d"--"full";
        mlet f2deltv : f2dElt <- r |> "f2d"--"elt";
